AwsCryptographicMaterialProviders/dafny/AwsCryptographyKeyStore/src/HierarchicalVersionUtils.dfy
@@ -217,4 +217,33 @@ module {:options "/functionSyntax:4" } HierarchicalVersionUtils {
     else
       Failure("Unable to decode string")
   }
+
+  // function HierarchyVersionToString(version: Types.HierarchyVersion): (output: string)
+  //   ensures output == Structure.HIERARCHY_VERSION_VALUE_1 || output == Structure.HIERARCHY_VERSION_VALUE_2
+  //   ensures StringToHierarchyVersion(output).Success? && StringToHierarchyVersion(output).value == version
+  // {
+  //   match version {
+  //     case v1 => Structure.HIERARCHY_VERSION_VALUE_1
+  //     case v2 => Structure.HIERARCHY_VERSION_VALUE_2
+  //   }
+  // }
+
+  // function StringToHierarchyVersion(version: string): (output: Result<Types.HierarchyVersion, Types.Error>)
+  //   ensures version == Structure.HIERARCHY_VERSION_VALUE_1 ==> output.Success? && output.value.v1?
+  //   ensures version == Structure.HIERARCHY_VERSION_VALUE_2 ==> output.Success? && output.value.v2?
+  //   ensures version != Structure.HIERARCHY_VERSION_VALUE_1 && version != Structure.HIERARCHY_VERSION_VALUE_2 ==> output.Failure?
+  // {
+  //   match version
+  //   case HIERARCHY_VERSION_VALUE_1 => Success(Types.HierarchyVersion.v1)
+  //   case HIERARCHY_VERSION_VALUE_2 => Success(Types.HierarchyVersion.v2)
+  //   case _ => Failure(Types.KeyStoreException(
+  //                       message := KeyStoreErrorMessages.INVALID_HIERARCHY_VERSION
+  //                     ))
+  // }
+
+  // lemma HierarchyVersionRoundTrip(version: Types.HierarchyVersion)
+  //   ensures StringToHierarchyVersion(HierarchyVersionToString(version)).Success?
+  //   ensures StringToHierarchyVersion(HierarchyVersionToString(version)).value == version
+  // {
+  // }
 }
